

# Chapter 4

## Moments and Moment Generating Functions

**Prof. N. G. J. Dias**

**Senior Professor and Head**

**Department of Computer Systems Engineering**

**Faculty of Computing and Technology**

**University of Kelaniya**

## 4.1 Introduction

- In this chapter we define a third special mathematical expectation, called the *moment generating function* (abbreviated mgf) of a random variable.
- The obvious purpose of the moment-generating function is in determining moments of random variables.
- However, the most important contribution is to establish distributions of functions of random variables.

## 2.2 Moments

- The following Definition 1 yields an expected value called the *rth moment about the mean* of the random variable  $X$ , which we denote by  $\mu_r$ .

- Definition 1 – Moment about the Mean

The *rth moment of a random variable  $X$  about the mean  $\mu$* , also called the *rth central moment*, is defined as

$$\mu_r = E[(X - \mu)^r],$$

where  $r = 0, 1, 2, \dots$ .

- We have,

$$\mu_r = E[(X - \mu)^r] = \begin{cases} \sum_x (x - \mu)^r f(x), & \text{if } X \text{ is discrete,} \\ \int_{-\infty}^{\infty} (x - \mu)^r f(x) dx, & \text{if } X \text{ is continuous.} \end{cases}$$

- It follows that  $\mu_0 = 1, \mu_1 = 0$  and  $\mu_2 = \sigma^2$ , i.e., the second central moment or second moment about the mean is the variance,  $Var(X)$  of  $X$ .
- The following Definition 2 yields an expected value called the *rth moment about the origin* of the random variable  $X$ , which we denote by  $\mu'_r$ .

- Definition 2 – Moment about the Origin

The *rth moment of a random variable  $X$  about the origin* is defined as

$$\mu'_r = E[X^r],$$

where  $r = 0, 1, 2, \dots$ .

- We have,

$$\mu'_r = E[X^r] = \begin{cases} \sum_x x^r f(x), & \text{if } X \text{ is discrete,} \\ \int_{-\infty}^{\infty} x^r f(x) dx, & \text{if } X \text{ is continuous.} \end{cases}$$

- Note that, the expected value of  $X$ ,  $E(X)$  is the first moment about the origin, i.e.,  $\mu'_1 = \mu$ .

- It can be shown that, the relationship between these moments is given by

$$\mu_r = \mu'_r - \binom{r}{1}\mu'_{r-1}\mu + \cdots + (-1)^i\binom{r}{i}\mu'_{r-i}\mu^i + \cdots + (-1)^r\mu'_0\mu^r.$$

As special cases we have, using  $\mu'_1 = \mu$  and  $\mu'_0 = 1$ ,

$$\mu_1 = \mu'_1 - \mu'_0\mu = \mu - \mu = 0,$$

$$\mu_2 = \mu'_2 - \mu^2,$$

$$\mu_3 = \mu'_3 - 3\mu'_2\mu + 2\mu^3,$$

$$\mu_4 = \mu'_4 - 4\mu'_3\mu + 6\mu'_2\mu^2 - 3\mu^4.$$

## 4.2 Moment Generating Functions

### 4.2.1 Defining Moment Generating Functions

- Although the moments of a random variable can be determined directly from Definition 1 and 2, an alternative procedure exists.
- This procedure requires us to utilize a *moment-generating function*.
- Definition 3 – Moment Generating Function (MGF)

The *moment-generating function* of the random variable  $X$  is denoted as  $M_X(t)$  and given by  $M_X(t) = E(e^{tX})$ , that is,

$$M_X(t) = \begin{cases} \sum_x e^{tx} f(x), & \text{if } X \text{ is discrete,} \\ \int_{-\infty}^{\infty} e^{tx} f(x) dx, & \text{if } X \text{ is continuous.} \end{cases}$$

Where no confusion can result we often write  $M(t)$  instead of  $M_X(t)$ .

- Moment-generating functions will exist only if the sum or integral of Definition 3 converges, i.e., as long as the sum or integral is finite for some interval of  $t$  around 0.

That is,  $M_X(t)$  is the MGF of  $X$  if there is a positive number  $h$  such that the above sum or integral exists and is finite for  $-h < t < h$ .

- When a moment-generating function  $M_X(t)$  of a random variable  $X$  does exist, we can derive the Taylor series expansion of the moment generating function  $M_X(t)$  as follows:

$$\begin{aligned}
 M_X(t) &= E(e^{tX}) = E\left(1 + \frac{tX}{1!} + \frac{(tX)^2}{2!} + \frac{(tX)^3}{3!} + \dots + \frac{(tX)^r}{r!} + \dots\right) \\
 &= 1 + \frac{t}{1!}E(X) + \frac{t^2}{2!}E(X^2) + \frac{t^3}{3!}E(X^3) + \dots + \frac{t^r}{r!}E(X^r) + \dots \\
 &= 1 + \mu t + \mu'_2 \frac{t^2}{2!} + \mu'_3 \frac{t^3}{3!} + \dots + \mu'_r \frac{t^r}{r!} + \dots
 \end{aligned}$$

### 4.2.2 Deriving Moments from Moment Generating Function

- Since each moment is an expected value, and the definition of expected value involves either a sum (in the discrete case) or an integral (in the continuous case), it seems that the computation of moments could be tedious.
- If a moment-generating function of a random variable  $X$  does exist, it can be used to generate all the moments of that variable.

The method is described in Theorem 1 without proof.



- **Theorem 1**

Let  $X$  be a random variable with moment generating function  $M_X(t)$ .

Then the  $r$ th moment of the random variable  $X$  about the origin will be obtained by

$$\mu'_r = E(X^r) = \left. \frac{d^r M_X(t)}{dt^r} \right|_{t=0},$$

i.e.,  $\mu'_r$  is the  $r$ th derivative of  $M_X(t)$  with respect to  $t$ , evaluated at the point  $t = 0$ .

- **Note:** If a MGF exists for a random variable  $X$ , then

(1) The mean of  $X$  can be found by evaluating the first derivative of the MGF at  $t = 0$ , i.e.,  $\mu = E(X) = M'_X(0)$ .

(2) The variance of  $X$  can be found by evaluating the first and second derivatives of the MGF at  $t = 0$ , i.e.,

$$\sigma^2 = E(X^2) - [E(X)]^2 = M''_X(0) - [M'_X(0)]^2.$$

## Example 1

The random variable  $X$  can assume the values 1 and  $-1$  with probability  $\frac{1}{2}$  each.

Find (a) the moment generating function,

(b) the first four moments about the origin.

### Solution:

$$(a) M_X(t) = E(e^{tX}) = e^{t(1)} \left(\frac{1}{2}\right) + e^{t(-1)} \left(\frac{1}{2}\right) = \frac{1}{2}(e^t + e^{-t}).$$

$$(b) \text{ We have, } e^t = 1 + \frac{t}{1!} + \frac{t^2}{2!} + \cdots + \frac{t^r}{r!} + \cdots, \text{ and}$$

$$e^{-t} = 1 - \frac{t}{1!} + \frac{t^2}{2!} + \cdots + (-1)^r \frac{t^r}{r!} + \cdots.$$

$$\text{Then } M_X(t) = \frac{1}{2}(e^t + e^{-t}) = 1 + \frac{t^2}{2!} + \frac{t^4}{4!} + \cdots. \quad \text{--- (1)}$$

$$\text{We also know that, } M_X(t) = 1 + \mu t + \mu'_2 \frac{t^2}{2!} + \mu'_3 \frac{t^3}{3!} + \cdots + \mu'_r \frac{t^r}{r!} + \cdots. \quad \text{--- (2)}$$

Then, comparing (1) and (2), we have

$$\mu = 0, \mu'_2 = 1, \mu'_3 = 0, \mu'_4 = 1, \dots$$

The odd moments are all zero, and the even moments are all one.

## Example 2

A random variable  $X$  has density function given by

$$f(x) = \begin{cases} 2e^{-2x}, & x \geq 0, \\ 0, & x < 0. \end{cases}$$

Find (a) the moment generating function,  
(b) the first four moments about the origin.

### Solution:

$$\begin{aligned} \text{(a) } M_X(t) &= E(e^{tX}) = \int_{-\infty}^{\infty} e^{tx} f(x) dx = \int_0^{\infty} e^{tx} (2e^{-2x}) dx = 2 \int_0^{\infty} e^{(t-2)x} dx \\ &= \frac{2e^{(t-2)x}}{t-2} \Big|_0^{\infty} = \frac{2}{2-t}, \text{ assuming } t < 2. \end{aligned}$$

(b) If  $|t| < 2$  we have

$$\begin{aligned} \frac{2}{2-t} &= \frac{1}{1-t/2} = 1 + \left(\frac{t}{2}\right) + \left(\frac{t}{2}\right)^2 + \left(\frac{t}{2}\right)^3 + \left(\frac{t}{2}\right)^4 + \dots \\ &= 1 + \frac{t}{2} + \frac{t^2}{4} + \frac{t^3}{8} + \frac{t^4}{16} + \dots. \quad \text{--- (1)} \end{aligned}$$

We also know that,  $M_X(t) = 1 + \mu t + \mu'_2 \frac{t^2}{2!} + \mu'_3 \frac{t^3}{3!} + \cdots + \mu'_r \frac{t^r}{r!} + \cdots$ . --- (2)

Therefore, on comparing terms of (1) and (2), we get

$$\mu = \frac{1}{2}, \mu'_2 = \frac{1}{2}, \mu'_3 = \frac{3}{4}, \mu'_4 = \frac{3}{2}.$$

### Example 3

Find the first four moments

(a) about the origin, (b) about the mean,

for a random variable  $X$  having density function  $f(x) = \begin{cases} \frac{4x(9-x^2)}{81}, & 0 \leq x \leq 3, \\ 0, & \text{otherwise.} \end{cases}$

**Solution:**

$$(a) \mu'_1 = E(X) = \int_0^3 \frac{4}{81} x \cdot x(9 - x^2) dx = \frac{4}{81} \int_0^3 x^2(9 - x^2) dx = \frac{8}{5} = \mu,$$

$$\mu'_2 = E(X^2) = \int_0^3 \frac{4}{81} x^2 \cdot x(9 - x^2) dx = \frac{4}{81} \int_0^3 x^3(9 - x^2) dx = 3,$$

$$\mu'_3 = E(X^3) = \int_0^3 \frac{4}{81} x^3 \cdot x(9 - x^2) dx = \frac{4}{81} \int_0^3 x^4(9 - x^2) dx = \frac{216}{35}, \text{ and}$$

$$\mu'_4 = E(X^4) = \int_0^3 \frac{4}{81} x^4 \cdot x(9 - x^2) dx = \frac{4}{81} \int_0^3 x^5(9 - x^2) dx = \frac{27}{2}.$$

(b) Using the results on slide 5,

$$\mu_1 = 0,$$

$$\mu_2 = \mu'_2 - \mu^2 = 3 - \left(\frac{8}{5}\right)^2 = \frac{11}{25} = \sigma^2,$$

$$\mu_3 = \mu'_3 - 3\mu'_2\mu + 2\mu^3 = \frac{216}{35} - 3 \cdot (3) \cdot \left(\frac{8}{5}\right) + 2 \cdot \left(\frac{8}{5}\right)^3 = -\frac{32}{875},$$

$$\begin{aligned}\mu_4 &= \mu'_4 - 4\mu'_3\mu + 6\mu'_2\mu^2 - 3\mu^4 \\ &= \frac{27}{2} - 4 \cdot \left(\frac{216}{35}\right) \cdot \left(\frac{8}{5}\right) + 6 \cdot (3) \cdot \left(\frac{8}{5}\right)^2 - 3 \cdot \left(\frac{8}{5}\right)^4 \\ &= \frac{3693}{8750}.\end{aligned}$$

### Example 4

Find the moment generating function of the binomial random variable  $X$  and then use it to verify that  $\mu = np$  and  $\sigma^2 = npq$ , where  $q = 1 - p$ .

**Solution:** We know that the probability distribution of the binomial random variable  $X$  is given by  $f(x) = P(X = x) = \binom{n}{x} p^x q^{n-x}$ .

$$\begin{aligned}\text{Thus, } M_X(t) &= E(e^{tX}) = \sum_{x=0}^n e^{tx} f(x) = \sum_{x=0}^n e^{tx} \binom{n}{x} p^x q^{n-x} \\ &= \sum_{x=0}^n \binom{n}{x} (pe^t)^x q^{n-x}.\end{aligned}$$

Recognizing this last sum as the binomial expansion of  $(pe^t + q)^n$ , we obtain

$$M_X(t) = (pe^t + q)^n.$$

$$\text{Now, } \frac{dM_X(t)}{dt} = n(pe^t + q)^{n-1} pe^t, \text{ and}$$

$$\frac{d^2 M_X(t)}{dt^2} = np[e^t(n-1)(pe^t + q)^{n-2} pe^t + (pe^t + q)^{n-1} e^t].$$



Setting  $t = 0$ , we get

$$\mu'_1 = np \text{ and } \mu'_2 = np[(n-1)p + 1].$$

Therefore,  $\mu = \mu'_1 = np$  and

$$\sigma^2 = \mu'_2 - \mu^2 = np[(n-1)p + 1] - (np)^2 = np(1-p) = npq.$$

## Exercises

1. The random variable  $X$  can assume the values  $\frac{1}{2}$  and  $-\frac{1}{2}$  with probability  $\frac{1}{2}$  each.  
Find (a) the moment generating function,  
(b) the first four moments about the origin.

2. Find the moment generating function of a random variable having density function

$$f(x) = \begin{cases} \frac{x}{2}, & 0 \leq x \leq 2, \\ 0, & \text{otherwise.} \end{cases}$$

Determine the first four moments about the origin.

3. Find the moment generating function of a random variable  $X$  having density function

$$f(x) = \begin{cases} e^{-x}, & x \geq 0, \\ 0, & \text{otherwise.} \end{cases}$$

Determine the moment generating function of  $X$  and the first four moments about the origin.

4. Let  $X$  have density function  $f(x) = \begin{cases} \frac{1}{b-a}, & a \leq x \leq b, \\ 0, & \text{otherwise.} \end{cases}$ . Find the  $k$ th moment about (a) the origin, (b) the mean.

5. Let  $f(x) = \begin{cases} \left(\frac{1}{2}\right)^x, & x = 1, 2, \dots, \\ 0, & \text{elsewhere} \end{cases}$ , be the pdf of the random variable  $X$ . Find the MGF, mean and the variance of  $X$ .

6. For each of the following pdfs, compute  $P(\mu - 2\sigma < X < \mu + 2\sigma)$ .

$$(a) f(x) = \begin{cases} 6x(1-x), & 0 < x < 1, \\ 0, & \text{elsewhere.} \end{cases} \quad (b) g(x) = \begin{cases} \left(\frac{1}{2}\right)^x, & x = 1, 2, \dots, \\ 0, & \text{elsewhere.} \end{cases}$$

### 4.2.3 Some Theorems on Moment Generating Functions

- Theorem 2 (Uniqueness Theorem)

Let  $X$  and  $Y$  be two random variables with moment generating functions  $M_X(t)$  and  $M_Y(t)$ , respectively.

If  $M_X(t) = M_Y(t)$  for all values of  $t$ , then  $X$  and  $Y$  have the same probability distribution.

- Theorem 3

Let  $X$  be a random variable with moment generating functions  $M_X(t)$  and let  $a$  be a constant. Then  $M_{X+a}(t) = e^{at} M_X(t)$ .

**Proof:**  $M_{X+a}(t) = E(e^{t(X+a)}) = e^{at} E(e^{tX}) = e^{at} M_X(t)$ .

- Theorem 4

Let  $X$  be a random variable with moment generating functions  $M_X(t)$  and let  $a$  be a constant. Then  $M_{aX}(t) = M_X(at)$ .

**Proof:**  $M_{aX}(t) = E(e^{t(aX)}) = E(e^{(at)X}) = M_X(at)$ .

- Theorem 5

Let  $X$  be a random variable with moment generating functions  $M_X(t)$  and let  $a$  and  $b(b \neq 0)$  be constants.

Then  $M_{(X+a)/b}(t) = e^{\frac{at}{b}} M_X\left(\frac{t}{b}\right)$ .

**Proof:**  $M_{(X+a)/b}(t) = E\left(e^{t\left(\frac{X+a}{b}\right)}\right) = e^{\frac{at}{b}} E\left(e^{\left(\frac{t}{b}\right)X}\right) = e^{\frac{at}{b}} M_X\left(\frac{t}{b}\right)$ .